src/program_proof/session/processClientRequest.v
@@ -5,16 +5,16 @@ Section heap.
   Context `{hG: !heapGS Σ}.
 
   Lemma wp_deleteAtIndexOperation (s: Slice.t) (index: w64) (l: list Operation.t) (n: nat) :
-      {{{
-            ⌜0 <= uint.nat index < length l⌝ ∗   
-            operation_slice s l n
-      }}}
-        deleteAtIndexOperation s #index
-        {{{
-              (ns: Slice.t), RET slice_val (ns);
-              operation_slice ns (coq_deleteAtIndexOperation l (uint.nat index)) n
-        }}}.
-  Proof.
+    {{{
+        ⌜0 <= uint.nat index < length l⌝ ∗   
+        operation_slice s l n
+    }}}
+      deleteAtIndexOperation s #index
+    {{{
+        (ns: Slice.t), RET slice_val (ns);
+        operation_slice ns (coq_deleteAtIndexOperation l (uint.nat index)) n
+    }}}.
+  Proof. (*
     iIntros (Φ) "(%H & H) H2".
     unfold deleteAtIndexOperation.
     wp_pures.
@@ -45,32 +45,31 @@ Section heap.
       + assert ((W64 1) = (w64_word_instance.(word.sub) (w64_word_instance.(word.add) index (W64 1)) (index))) by word. rewrite H0. destruct (slice_skip_skip (w64_word_instance.(word.add) index (W64 1)) index s (struct.t Operation)); try word. rewrite <- H0. iApply "H7".
     - iIntros (s''') "[H H6]". wp_pures. iApply "H2".
       iExists (([] ++ take (uint.nat index) ops) ++ drop (uint.nat (W64 1)) (drop (uint.nat index) ops)). simpl.
-      iSplit.
+      iSplit. *)
   Admitted.
 
-  (*
   Lemma wp_deleteAtIndexMessage (s: Slice.t) (index: w64) (l: list Message.t) (n: nat) :
-      {{{
-            ⌜0 <= uint.nat index < length l⌝ ∗   
-            message_slice s l n
-      }}}
-        deleteAtIndexMessage s #index
-        {{{
-              (ns: Slice.t), RET slice_val (ns);
-              message_slice ns (coq_deleteAtIndexMessage l (uint.nat index)) n
-        }}}.
+    {{{
+      ⌜0 <= uint.nat index < length l⌝ ∗   
+      message_slice s l n
+    }}}
+      deleteAtIndexMessage s #index
+    {{{
+        (ns: Slice.t), RET slice_val (ns);
+        message_slice ns (coq_deleteAtIndexMessage l (uint.nat index)) n
+    }}}.
   Proof.
-   *)
+  Admitted.
   
   Lemma wp_getDataFromOperationLog (s: Slice.t) (l: list Operation.t) (n: nat) :
     {{{
-          operation_slice s l n
+        operation_slice s l n
     }}}
       getDataFromOperationLog s
-      {{{
-            r , RET #r;
-            ⌜r = coq_getDataFromOperationLog l⌝
-      }}}.
+    {{{
+        r , RET #r;
+        ⌜r = coq_getDataFromOperationLog l⌝
+    }}}.
   Proof.
   Admitted.
 
@@ -80,11 +79,24 @@ Section heap.
           is_operation opv2 o2 n
     }}}
       equalOperations (operation_val opv1) (operation_val opv2)
-      {{{ r , RET #r;
-          ⌜r = coq_equalOperations o1 o2⌝
+    {{{ r , RET #r;
+        ⌜r = coq_equalOperations o1 o2⌝
+    }}}.
+  Proof.
+  Admitted.
+
+  Lemma wp_mergeOperations (s1 s2: Slice.t) (l1 l2: list Operation.t) (n: nat) :
+    {{{
+          operation_slice s1 l1 n ∗
+          operation_slice s2 l2 n 
+    }}}
+      mergeOperations s1 s2 
+      {{{
+            (ns: Slice.t), RET slice_val (ns);
+            ∃ nxs, operation_slice ns nxs n ∗
+                   ⌜nxs = coq_mergeOperations l1 l2⌝
       }}}.
   Proof.
   Admitted.
 
-  
 End heap.
